\documentclass{article}
\usepackage{amsmath}  % DeclareMathOperator
\usepackage{amssymb}  % mathbb
\usepackage{mathtools}

\DeclareMathOperator{\ran}{ran}

\begin{document}
\section{Chapter 6}
\subsection{4.}
Let $f:[0, 1] \to (0, 1)$ be defined by
\begin{equation}
  f(x) = 
  \begin{cases}
    2^{-1} &\text{if } x=0; \\
    2^{-2} &\text{if } x=2^0; \\
    2^{-3} &\text{if } x=2^{-1}; \\
    \vdotswithin{ 2^{-3}}\\
    x & \text{otherwise}.
  \end{cases}
\end{equation}

We want to show that if $f(a) = y$ and $f(b) = y$,
then $a = b$.
If $y = 2^{-1}$, then $a = b = 0$.
If $y = 2^{-2}, 2^{-3}, dots$, then  $a = b = 2^0, 2^{-1}, \dots$.
Otherwise, $y = a = b$.


\end{document}